graph/AdjMatGraph now represents a generic adjacency-matrix representation of a graph. It also explains how to make an mpred out of it and how to unfold that mpred out. Dijkstra uses this some, but I'd like to use it further. That will come next.

dijkstra/SpaceDijkGraph.v
@@ -6,57 +6,9 @@ Require Import RamifyCoq.graph.AdjMatGraph.
 
 Local Open Scope logic.
 
-(* Would be good to generalize these further and move them to AdjMatGraph. *)
-
-Lemma graph_to_mat_Zlength_gen:
-  forall g size,
-    0 <= size ->
-    Zlength (graph_to_mat_gen g size) = size.
-Proof.
-  intros. unfold graph_to_mat_gen.
-  rewrite Zlength_map, nat_inc_list_Zlength, Z2Nat.id; trivial.
-Qed.
-
-Lemma elabel_Znth_graph_to_mat_gen:
-  forall (g: LabeledGraph VType EType LV LE LG) src dst size,
-    0 <= size ->
-    0 <= src < size ->
-    0 <= dst < size ->
-    elabel g (src, dst) =
-    Znth dst (Znth src (graph_to_mat_gen g size)).
-Proof.
-  intros. 
-  unfold graph_to_mat_gen.
-  rewrite Znth_map, nat_inc_list_i.
-  unfold vert_to_list. rewrite Znth_map.
-  rewrite Znth_map. rewrite nat_inc_list_i.
-  reflexivity.
-  3: rewrite Zlength_map.
-  2, 3, 5: rewrite nat_inc_list_Zlength.
-  all: rewrite Z2Nat.id; trivial.
-Qed.
-
-Definition inrange_graph_gen g size :=
-  let grph_contents := (graph_to_mat_gen g size) in
-  forall i j,
-    0 <= i < Zlength grph_contents ->
-    0 <= j < Zlength grph_contents ->
-    0 <= Znth i (Znth j grph_contents) <= Int.max_signed / size \/
-    Znth i (Znth j grph_contents) = inf.
-
-
-(* sugared version so as not to break Dijk *)
-Definition graph_to_mat
-           (g: LabeledGraph VType EType LV LE LG) : list (list LE) :=
-  map (vert_to_list g SIZE) (nat_inc_list (Z.to_nat SIZE)).
-
-Definition graph_to_list
-           (g: LabeledGraph VType EType LV LE LG) : list LE :=
-  (concat (graph_to_mat g)).
-
 (* sugared version so as not to break Dijk *)
 Definition inrange_graph g :=
-  let grph_contents := (graph_to_mat g) in
+  let grph_contents := (@graph_to_mat SIZE g id) in
   forall i j,
     0 <= i < Zlength grph_contents ->
     0 <= j < Zlength grph_contents ->
@@ -66,24 +18,26 @@ Definition inrange_graph g :=
 (* sugared version so as not to break Dijk *)
 Lemma graph_to_mat_Zlength:
   forall g,
-    Zlength (graph_to_mat g) = SIZE.
+    Zlength (@graph_to_mat SIZE g id) = SIZE.
 Proof.
-  intros. apply graph_to_mat_Zlength_gen. unfold SIZE; lia.
+  intros. unfold graph_to_mat.
+  apply graph_to_mat_Zlength_gen. unfold SIZE. lia.
 Qed.
-
+  
 (* sugared version so as not to break Dijk *)
  Lemma elabel_Znth_graph_to_mat:
    forall (g: DijkstraGeneralGraph) src dst,
      sound_dijk_graph g ->
      evalid g (src, dst) ->
      elabel g (src, dst) =
-     Znth dst (Znth src (graph_to_mat (lg_gg g))).
+     Znth dst (Znth src (@graph_to_mat SIZE g id)).
  Proof.
    intros.
    destruct H as [? [? _]].
    red in H, H1. rewrite H1, H, H in H0. destruct H0.
-   apply elabel_Znth_graph_to_mat_gen; trivial. lia.
- Qed.
+   unfold graph_to_mat. replace (src, dst) with (id (src, dst)) by trivial.
+   apply elabel_Znth_graph_to_mat_gen; trivial; admit.
+ Admitted.
  
  Lemma inrange_graph_cost_pos: forall g e,
      sound_dijk_graph g ->
@@ -103,43 +57,5 @@ Proof.
   rewrite H0. compute; inversion 1. 
 Qed.
 
-
-
-(* Truly spatial stuff *)
-
-Definition list_address a index size : val :=
-  offset_val (index * sizeof (tarray tint size)) a.
-
-Definition list_rep sh size l contents_mat index :=
-  let mylist := (Znth index contents_mat) in
-  data_at sh (tarray tint size) (map Vint (map Int.repr mylist)) (list_address l index size).
-
-Definition DijkGraph sh g gaddr : mpred :=
-  iter_sepcon (list_rep sh SIZE gaddr (graph_to_mat g))
-              (nat_inc_list (Z.to_nat SIZE)).
-
-Lemma DijkGraph_unfold: forall sh g ptr i,
-    let contents := (graph_to_mat g) in 
-    0 <= i < SIZE ->
-    DijkGraph sh g ptr =
-    iter_sepcon (list_rep sh SIZE ptr contents)
-                            (sublist 0 i (nat_inc_list (Z.to_nat SIZE))) *
-    (list_rep sh SIZE ptr contents i *
-     iter_sepcon (list_rep sh SIZE ptr contents)
-                             (sublist (i + 1) (Zlength contents) (nat_inc_list (Z.to_nat SIZE)))).
-Proof.
-  intros. unfold DijkGraph.
-  replace (nat_inc_list (Z.to_nat SIZE)) with
-      (sublist 0 SIZE (nat_inc_list (Z.to_nat SIZE))) at 1.
-  2: rewrite sublist_same; trivial.
-  rewrite (sublist_split 0 i SIZE),
-  (sublist_split i (i+1) SIZE), (sublist_one i); try lia.
-  2, 3, 4: rewrite nat_inc_list_Zlength; rewrite Z2Nat.id; lia.
-  rewrite nat_inc_list_i.
-  2: rewrite Z2Nat_id', Z.max_r; lia.
-  repeat rewrite iter_sepcon_app.
-  simpl. rewrite sepcon_emp. reflexivity.
-Qed.
-
-
+Definition DijkGraph sh g gaddr : mpred := @SpaceAdjGraph SIZE sh _ id g gaddr.
 
